Ok epsilon is fixed, ready to dive into the beast

theories/Eq/Epsilon.v
@@ -1,8 +1,8 @@
 (* begin hide *)
 
 From ITree Require Import
-     Basics.Basics
-     Core.Subevent.
+  Basics.Basics
+  Core.Subevent.
 
 From CTree Require Import
   CTree
@@ -16,69 +16,70 @@ Open Scope ctree_scope.
 (*|
 Helper inductive: [epsilon_det t t'] judges that [t' ≡ Guard* t]
 |*)
-  Inductive epsilon_det {E C X} `{B1 -< C}: relation (ctree E C X) :=
+  Inductive epsilon_det {E C X}: relation (ctree E C X) :=
   | epsilon_det_id : forall t t', t ≅ t' -> epsilon_det t t'
-  | epsilon_det_tau : forall t t' t'',
+  | epsilon_det_guard : forall t t' t'',
       epsilon_det t t' -> t'' ≅ Guard t -> epsilon_det t'' t'.
 
 (*|
-Helper inductive: [productive t] judges that [t]'s head constructor is not a [BrD]
+Helper inductive: [productive t] judges that [t]'s head constructor is not a [Br]
 |*)
   Inductive productive {E C X} : ctree E C X -> Prop :=
   | prod_ret {r t} (EQ: t ≅ Ret r) : productive t
   | prod_vis {Y} {e : E Y} {k t} (EQ: t ≅ Vis e k) : productive t
-  | prod_tau {X} {c: C X} {k t} (EQ: t ≅ BrS c k) : productive t.
+  | prod_step {t u} (EQ: t ≅ Step u) : productive t.
 
 (*|
-Helper inductive: [epsilon t t'] judges that [t'] is reachable from [t] by a path made of [BrD] branches.
+Helper inductive: [epsilon t t'] judges that [t'] is reachable from [t] by a path made of [Br] branches.
 |*)
   Inductive epsilon_ {E C X} : ctree' E C X -> ctree' E C  X -> Prop :=
-  | EpsilonId : forall t t', t ≅ t' -> epsilon_ (observe t) (observe t')
-  | EpsilonBr : forall X (c: C X) k x t, epsilon_ (observe (k x)) t -> epsilon_ (BrDF c k) t.
+  | epsilon_id : forall t t', t ≅ t' -> epsilon_ (observe t) (observe t')
+  | epsilon_br : forall X (c: C X) k x t, epsilon_ (observe (k x)) t -> epsilon_ (BrF c k) t
+  | epsilon_guard : forall t u, epsilon_ (observe u) t -> epsilon_ (GuardF u) t.
 
   Definition epsilon {E C X} (t t' : ctree E C X) := epsilon_ (observe t) (observe t').
 
   Section epsilon_det_theory.
 
-    #[global] Instance epsilon_det_equ {E C X} `{Tau: B1 -< C}:
-    Proper (equ eq ==> equ eq ==> flip impl) (@epsilon_det E C X _).
+    #[global] Instance epsilon_det_equ {E C X}:
+    Proper (equ eq ==> equ eq ==> flip impl) (@epsilon_det E C X).
     Proof.
       cbn. intros.
       revert x H. induction H1; intros.
       - econstructor. now rewrite H0, H1.
-      - eapply epsilon_det_tau. apply IHepsilon_det. apply H0. reflexivity. rewrite H2. apply H.
+      - eapply epsilon_det_guard. apply IHepsilon_det. apply H0. reflexivity. rewrite H2. apply H.
     Qed.
 
-    #[global] Instance epsilon_det_equ' {E C X} `{Tau: B1 -< C}:
-      Proper (equ eq ==> equ eq ==> impl) (@epsilon_det E C X _).
+    #[global] Instance epsilon_det_equ' {E C X}:
+      Proper (equ eq ==> equ eq ==> impl) (@epsilon_det E C X).
     Proof.
       cbn. intros. rewrite <- H, <- H0. apply H1.
     Qed.
 
-    #[global] Instance epsilon_det_refl {E C X} `{HasB1: B1 -< C} :
-      Reflexive (@epsilon_det E C X _).
+    #[global] Instance epsilon_det_refl {E C X} :
+      Reflexive (@epsilon_det E C X).
     Proof.
       now left.
     Qed.
 
-    #[global] Instance Transitive_epsilon_det {E C X} `{HasB1: B1 -< C} :
-      Transitive (@epsilon_det E C X _).
+    #[global] Instance Transitive_epsilon_det {E C X} :
+      Transitive (@epsilon_det E C X).
     Proof.
       cbn. intros. induction H.
       - now subs.
       - subs. eright. now apply IHepsilon_det. reflexivity.
     Qed.
 
-    Lemma epsilon_det_bind {E C X Y} `{Tau: B1 -< C}: forall (t t' : ctree E C X) (k : X -> ctree E C Y),
+    Lemma epsilon_det_bind {E C X Y}: forall (t t' : ctree E C X) (k : X -> ctree E C Y),
         epsilon_det t t' ->
         epsilon_det (t >>= k) (t' >>= k).
     Proof.
       intros. induction H.
-      - rewrite H. constructor. reflexivity.
-      - rewrite H0. setoid_rewrite bind_guard. eapply epsilon_det_tau. apply IHepsilon_det. reflexivity.
+      - setoid_rewrite H. constructor. reflexivity.
+      - rewrite H0. setoid_rewrite bind_guard. eapply epsilon_det_guard. apply IHepsilon_det. reflexivity.
     Qed.
 
-    Lemma epsilon_det_bind_ret_l {E C X Y} `{Tau: B1 -< C}: forall (t : ctree E C X) t' (k : X -> ctree E C Y) x,
+    Lemma epsilon_det_bind_ret_l {E C X Y}: forall (t : ctree E C X) t' (k : X -> ctree E C Y) x,
         epsilon_det t (Ret x) ->
         epsilon_det (k x) t' ->
         epsilon_det (t >>= k) t'.
@@ -86,20 +87,21 @@ Helper inductive: [epsilon t t'] judges that [t'] is reachable from [t] by a pat
       intros. remember (Ret x) as R. revert t' k x HeqR H0. induction H; intros; subst.
       - subst. rewrite H, bind_ret_l. apply H0.
       - rewrite H0. setoid_rewrite bind_guard.
-        eapply epsilon_det_tau. 2: reflexivity. eapply IHepsilon_det. reflexivity. apply H1.
+        eapply epsilon_det_guard. 2: reflexivity. eapply IHepsilon_det. reflexivity. apply H1.
     Qed.
 
-    Lemma epsilon_det_bind_ret_l_equ {E C X Y} `{Tau: B1 -< C}:
+    Lemma epsilon_det_bind_ret_l_equ {E C X Y}:
       forall (t : ctree E C X) (k : X -> ctree E C Y) x,
         epsilon_det t (Ret x) ->
         x <- t;; k x ≅ t;; k x.
     Proof.
       intros. remember (Ret x) as R. induction H; subst.
       - rewrite H. rewrite !bind_ret_l. reflexivity.
-      - rewrite H0. rewrite !bind_guard. apply br_equ. intro. apply IHepsilon_det. reflexivity.
+      - rewrite H0. rewrite !bind_guard. apply guard_equ.
+        apply IHepsilon_det. reflexivity.
     Qed.
 
-    Lemma epsilon_det_trans {E C X} `{Stuck: B0 -< C} `{Tau: B1 -< C} :
+    Lemma epsilon_det_trans {E C X} :
       forall l (t t' t'' : ctree E C X),
         epsilon_det t t' -> trans l t' t'' -> trans l t t''.
     Proof.
@@ -108,7 +110,7 @@ Helper inductive: [epsilon t t'] judges that [t'] is reachable from [t] by a pat
       - apply IHepsilon_det in H0. apply trans_guard in H0. now rewrite <- H1 in H0.
     Qed.
 
-    Lemma sbisim_epsilon_det {E C X} `{Stuck: B0 -< C} `{Tau: B1 -< C}:
+    Lemma sbisim_epsilon_det {E C X}:
       forall (t t' : ctree E C X), epsilon_det t t' -> t ~ t'.
     Proof.
       intros. induction H.
@@ -125,7 +127,7 @@ Helper inductive: [epsilon t t'] judges that [t'] is reachable from [t] by a pat
       cbn. intros. inv H0; rewrite H in *.
       - eapply prod_ret; eauto.
       - eapply prod_vis; eauto.
-      - eapply prod_tau; eauto.
+      - eapply prod_step; eauto.
     Qed.
 
     #[global] Instance productive_equ' : forall {E C X}, Proper (equ eq ==> flip impl) (@productive E C X).
@@ -136,20 +138,18 @@ Helper inductive: [epsilon t t'] judges that [t'] is reachable from [t] by a pat
     #[local] Hint Constructors productive : trans.
 
     Lemma ctree_case_productive : forall {E C X} (t: ctree E C X),
-      productive t \/ exists X (c : C X) k, t ≅ BrD c k.
+      productive t
+      \/ (exists X (c : C X) k, t ≅ Br c k)
+      \/ (exists u, t ≅ Guard u)
+      \/ t ≅ Stuck.
     Proof.
-      intros. setoid_rewrite (ctree_eta t). desobs t; etrans.
-      destruct vis; etrans.
+      intros. setoid_rewrite (ctree_eta t).
+      desobs t; etrans.
+      right; left; eauto 8.
     Qed.
 
-    Lemma productive_br {E C X Y} : forall vis c (k : Y -> ctree E C X),
-      productive (Br vis c k) -> vis = true.
-    Proof.
-      intros. inv H; inv_equ. reflexivity.
-    Qed.
-
-    Lemma productive_brD : forall {E C X Y} (c : C Y) (k : Y -> ctree E C X),
-      ~ productive (BrD c k).
+    Lemma productive_br : forall {E C X Y} (c : C Y) (k : Y -> ctree E C X),
+      ~ productive (Br c k).
     Proof.
       intros ** ?. inversion H; inv_equ.
     Qed.
@@ -158,18 +158,18 @@ Helper inductive: [epsilon t t'] judges that [t'] is reachable from [t] by a pat
     Proof.
       intros. inversion H; inv_equ; subst.
       - apply ret_equ_bind in EQ as (? & ? & ?). subs. now eapply prod_ret.
-      - apply vis_equ_bind in EQ as [(? & ?) | (? & ? & ?)]; subs.
+      - apply vis_equ_bind in EQ as [(? & ? & ?) | (? & ? & ?)]; subs.
         + now eapply prod_ret.
         + now eapply prod_vis.
-      - apply br_equ_bind in EQ as [(? & ?) | (? & ? & ?)]; subs.
+      - apply step_equ_bind in EQ as [(? & ? & ?) | (? & ? & ?)]; subs.
         + now eapply prod_ret.
-        + now eapply prod_tau.
+        + now eapply prod_step.
     Qed.
 
   End productive_theory.
 
   #[global] Hint Constructors productive : trans.
-  #[global] Hint Resolve productive_brD : trans.
+  #[global] Hint Resolve productive_br : trans.
 
   Section epsilon_theory.
 
@@ -178,11 +178,16 @@ Helper inductive: [epsilon t t'] judges that [t'] is reachable from [t] by a pat
     Proof.
       cbn. intros.
       revert y y0 H H0. induction H1; intros.
-      - pose (EpsilonId (go y) (go y0)). cbn in e. apply e.
+      - pose (epsilon_id (go y) (go y0)). cbn in e. apply e.
         rewrite <- H0, <- H1, H. reflexivity.
       - destruct H. step in H. inv H. invert.
         econstructor.
         apply IHepsilon_.
+        + constructor.
+          rewrite <- !ctree_eta. apply REL.
+        + apply H0.
+      - destruct H; step in H; inv H.
+        constructor; apply IHepsilon_.
         + constructor.
           rewrite <- !ctree_eta. apply REL.
         + apply H0.
@@ -204,47 +209,65 @@ Helper inductive: [epsilon t t'] judges that [t'] is reachable from [t] by a pat
     #[global] Instance epsilon_refl {E C X} :
       Reflexive (@epsilon E C X).
     Proof.
-      now left.
+      now constructor 1.
     Qed.
 
-    Lemma epsilon_br {E C X Y} : forall (t' : ctree E C X) k (c : C Y) x,
-      epsilon (k x) t' -> epsilon (BrD c k) t'.
+    Lemma epsilon_Br {E C X Y} : forall (t' : ctree E C X) k (c : C Y) x,
+      epsilon (k x) t' -> epsilon (Br c k) t'.
     Proof.
-      intros. eright. apply H.
+      intros. econstructor 2; apply H.
     Qed.
 
     Lemma epsilon_case {E C X} : forall (t t' : ctree E C X),
       epsilon t t' ->
-      t ≅ t' \/ exists Y (c : C Y) k x, t ≅ BrD c k /\ epsilon (k x) t'.
+      t ≅ t'
+      \/ (exists Y (c : C Y) k x, t ≅ Br c k /\ epsilon (k x) t')
+      \/ (exists u, t ≅ Guard u /\ epsilon u t').
     Proof.
       intros * EPS.
-      inversion EPS; [left | right].
+      inversion EPS; [left | right; left | right; right].
       - setoid_rewrite ctree_eta. now rewrite <- H, H1, H0.
       - subst. exists X0, c, k, x. split; auto. now rewrite H, <- ctree_eta.
+      - eexists; split; eauto.
+        now rewrite H, <- ctree_eta.
     Qed.
 
-    Lemma epsilon_trans {E C X} `{Stuck: B0 -< C} : forall (t t' : ctree E C X),
+    Lemma epsilon_trans {E C X} : forall (t t' : ctree E C X),
         epsilon t t' -> forall l t'', trans l t' t'' -> trans l t t''.
     Proof.
       intros. red in H. rewrite ctree_eta. rewrite ctree_eta in H0.
       genobs t ot. genobs t' ot'. clear t Heqot t' Heqot'.
       induction H.
       - rewrite H. apply H0.
-      - apply IHepsilon_ in H0. eapply trans_brD in H0. apply H0. rewrite <- ctree_eta. reflexivity.
+      - apply IHepsilon_ in H0. eapply trans_br in H0. apply H0. rewrite <- ctree_eta. reflexivity.
+      - apply IHepsilon_ in H0; etrans.
     Qed.
 
-    Lemma epsilon_fwd : forall {E C X} (t : ctree E C X) k x (c : C X),
-        epsilon t (BrD c k) -> epsilon t (k x).
+    Lemma epsilon_fwd : forall {E C X Y} (t : ctree E C X) k x (c : C Y),
+        epsilon t (Br c k) -> epsilon t (k x).
     Proof.
       intros. red in H. red.
       genobs t ot. clear t Heqot.
-      remember (observe (BrD c k)) as oc.
+      remember (observe (Br c k)) as oc.
       revert c k x Heqoc. induction H.
-      - intros. rewrite H, Heqoc. cbn. eapply EpsilonBr. econstructor. reflexivity.
-      - intros. subst. eapply EpsilonBr. eapply IHepsilon_. reflexivity.
+      - intros. rewrite H, Heqoc. cbn. eapply epsilon_br. econstructor. reflexivity.
+      - intros. subst. eapply epsilon_br. eapply IHepsilon_. reflexivity.
+      - intros; subst; eapply epsilon_guard, IHepsilon_; reflexivity.
     Qed.
 
-    Lemma trans_epsilon {E C X} `{Stuck: B0 -< C} l (t t'' : ctree E C X) : trans l t t'' -> exists t',
+    Lemma epsilon_fwd' : forall {E C X} (t u : ctree E C X),
+        epsilon t (Guard u) -> epsilon t u.
+    Proof.
+      intros. red in H. red.
+      genobs t ot. clear t Heqot.
+      remember (observe (Guard u)) as oc.
+      revert u Heqoc. induction H.
+      - intros. rewrite H, Heqoc. cbn. eapply epsilon_guard. econstructor. reflexivity.
+      - intros. subst. eapply epsilon_br. eapply IHepsilon_. reflexivity.
+      - intros; subst; eapply epsilon_guard, IHepsilon_; reflexivity.
+    Qed.
+
+    Lemma trans_epsilon {E C X} l (t t'' : ctree E C X) : trans l t t'' -> exists t',
           epsilon t t' /\ productive t' /\ trans l t' t''.
     Proof.
       intros. do 3 red in H.
@@ -252,24 +275,27 @@ Helper inductive: [epsilon t t'] judges that [t'] is reachable from [t] by a pat
       genobs t ot. genobs t'' ot''. clear t Heqot t'' Heqot''.
       induction H; intros.
       - destruct IHtrans_ as (? & ? & ? & ?).
-        rewrite <- ctree_eta in H0. eapply EpsilonBr in H0.
+        rewrite <- ctree_eta in H0. eapply epsilon_br in H0.
         exists x0. etrans.
+      - destruct IHtrans_ as (? & ? & ? & ?).
+        rewrite <- ctree_eta in H0. eapply epsilon_guard in H0.
+        eexists; etrans.
       - eexists. split; [| split ].
-        + left. reflexivity.
-        + eapply prod_tau. reflexivity.
+        + constructor 1. reflexivity.
+        + eapply prod_step. reflexivity.
         + rewrite <- H, <- ctree_eta. etrans.
       - eexists. split; [| split ].
-        + left. reflexivity.
+        + constructor 1. reflexivity.
         + eapply prod_vis. reflexivity.
         + rewrite <- H, <- ctree_eta. etrans.
       - eexists. split; [| split ].
-        + left. reflexivity.
+        + constructor 1. reflexivity.
         + eapply prod_ret. reflexivity.
-        + rewrite br0_always_stuck. etrans.
+        + etrans.
     Qed.
 
-    Lemma trans_val_epsilon {E C X}  `{Stuck: B0 -< C}  : forall x (t t' : ctree E C X),
-        trans (val x) t t' -> epsilon t (Ret x) /\ t' ≅ stuckD.
+    Lemma trans_val_epsilon {E C X} : forall x (t t' : ctree E C X),
+        trans (val x) t t' -> epsilon t (Ret x) /\ t' ≅ Stuck.
     Proof.
       intros. apply trans_epsilon in H as (? & ? & ? & ?).
       inv H0.
@@ -278,20 +304,18 @@ Helper inductive: [epsilon t t'] judges that [t'] is reachable from [t] by a pat
       - rewrite EQ in H1. inv_trans.
     Qed.
 
-    Lemma trans_tau_epsilon {E C X}  `{Stuck: B0 -< C} : forall (t t' : ctree E C X),
-        trans tau t t' -> exists X (c: C X) k x, epsilon t (BrS c k) /\ t' ≅ k x.
+    Lemma trans_τ_epsilon {E C X} : forall (t t' : ctree E C X),
+        trans τ t t' -> exists u, epsilon t (Step u) /\ t' ≅ u.
     Proof.
       intros. apply trans_epsilon in H as (? & ? & ? & ?).
       inv H0.
       - rewrite EQ in H1. inv_trans.
       - rewrite EQ in H1. inv_trans.
       - rewrite EQ in H1. inv_trans.
-        do 2 eexists.
-        exists k. exists x0.
         eauto.
     Qed.
 
-    Lemma trans_obs_epsilon {E C X Y} `{Stuck: B0 -< C} : forall (t t' : ctree E C X) e (x : Y),
+    Lemma trans_obs_epsilon {E C X Y} : forall (t t' : ctree E C X) e (x : Y),
         trans (obs e x) t t' -> exists k, epsilon t (Vis e k) /\ t' ≅ k x.
     Proof.
       intros. apply trans_epsilon in H as (? & ? & ? & ?).
@@ -306,12 +330,8 @@ Helper inductive: [epsilon t t'] judges that [t'] is reachable from [t] by a pat
     Proof.
       intros. setoid_rewrite ctree_eta.
       inversion H; subst; rewrite (ctree_eta t) in EQ; inversion H0; subst.
-      - now rewrite H3.
-      - rewrite <- H1 in EQ. step in EQ. inv EQ.
-      - now rewrite H3.
-      - rewrite <- H1 in EQ. step in EQ. inv EQ.
-      - now rewrite H3.
-      - rewrite <- H1 in EQ. step in EQ. inv EQ.
+      all: try now rewrite H3.
+      all: try now (rewrite <- H1 in EQ; step in EQ; inv EQ).
     Qed.
 
     #[global] Instance epsilon_transitive {E C X} : Transitive (@epsilon E C X).
@@ -322,7 +342,9 @@ Helper inductive: [epsilon t t'] judges that [t'] is reachable from [t] by a pat
       revert v H0. induction H; intros.
       - subs. apply H0.
       - setoid_rewrite <- ctree_eta in IHepsilon_.
-        eright. now apply IHepsilon_.
+        econstructor 2. now apply IHepsilon_.
+      - setoid_rewrite <- ctree_eta in IHepsilon_.
+        econstructor 3. now apply IHepsilon_.
     Qed.
 
     Lemma epsilon_bind_l {E C X Y} : forall t t' (k : Y -> ctree E C X),
@@ -332,7 +354,8 @@ Helper inductive: [epsilon t t'] judges that [t'] is reachable from [t] by a pat
       red in H. genobs t ot. genobs t' ot'. clear t Heqot t' Heqot'.
       induction H.
       - subs. reflexivity.
-      - rewrite bind_br. eright. rewrite (ctree_eta (k0 x)). apply IHepsilon_.
+      - rewrite bind_br. econstructor 2. rewrite (ctree_eta (k0 x)). apply IHepsilon_.
+      - rewrite bind_guard. econstructor 3; eauto.
     Qed.
 
     Lemma epsilon_bind_ret {E C X Y} : forall t (k : Y -> ctree E C X) v,
@@ -363,22 +386,32 @@ Helper inductive: [epsilon t t'] judges that [t'] is reachable from [t] by a pat
       - setoid_rewrite (ctree_eta t0) in H0. destruct (observe t0) eqn:?; inv_equ.
         + right. exists r. split; auto.
           rewrite bind_ret_l in H0. rewrite <- H0. apply epsilon_br with (x := x). apply H.
-        + rewrite bind_br in H0. inv_equ.
+        + rewrite bind_br in H0.
+          inv_equ.
           setoid_rewrite <- ctree_eta in IHepsilon_.
           apply IHepsilon_ in EQ. destruct EQ as [(? & ? & ?) | (? & ? & ?)].
           * left. exists x0. split; auto. eapply epsilon_br; eassumption.
           * right. exists x0. split; auto. eapply epsilon_br; eassumption.
+      - setoid_rewrite (ctree_eta t0) in H0. destruct (observe t0) eqn:?; inv_equ.
+        + right. exists r. split; auto.
+          rewrite bind_ret_l in H0. rewrite <- H0. apply epsilon_guard, H.
+        + rewrite bind_guard in H0.
+          inv_equ.
+          setoid_rewrite <- ctree_eta in IHepsilon_.
+          apply IHepsilon_ in H0. destruct H0 as [(? & ? & ?) | (? & ? & ?)].
+          * left. exists x. split; auto. eapply epsilon_guard; eassumption.
+          * right. exists x. split; auto. eapply epsilon_guard; eassumption.
     Qed.
 
-    Lemma epsilon_det_epsilon {E C X} `{Stuck: B0 -< C} `{Tau: B1 -< C} : forall (t t' : ctree E C X),
+    Lemma epsilon_det_epsilon {E C X} : forall (t t' : ctree E C X),
         epsilon_det t t' -> epsilon t t'.
     Proof.
       intros. induction H.
-      - now left.
-      - rewrite H0. now right.
+      - now constructor.
+      - rewrite H0. now constructor.
     Qed.
 
-    Lemma ss_epsilon_l {E F C D X Y L R} `{Stuck: B0 -< C} `{Stuck': B0 -< D}
+    Lemma ss_epsilon_l {E F C D X Y L R}
         (t t0 : ctree E C X) (u : ctree F D Y) :
       epsilon t0 t ->
       ss L R t0 u ->
@@ -390,7 +423,7 @@ Helper inductive: [epsilon t t'] judges that [t'] is reachable from [t] by a pat
     Qed.
 
     (* Is this one really useful? *)
-    Lemma ss_epsilon_l' {E F C D X Y L R} `{Stuck: B0 -< C} `{Stuck': B0 -< D}
+    Lemma ss_epsilon_l' {E F C D X Y L R}
         (t : ctree E C X) (u : ctree F D Y) :
       (forall t0, epsilon t t0 -> productive t0 -> ss L R t0 u) ->
       ss L R t u.
@@ -400,12 +433,13 @@ Helper inductive: [epsilon t t'] judges that [t'] is reachable from [t] by a pat
       setoid_rewrite (ctree_eta t) in H. genobs t ot. clear t Heqot.
       rewrite (ctree_eta x) in H1, H2. genobs x ox. clear x Heqox.
       induction H0.
-      - apply H in H1 as ?. 2: { rewrite H0. now left. }
+      - apply H in H1 as ?. 2: { rewrite H0. now constructor. }
         apply H3 in H2. apply H2.
-      - apply IHepsilon_; auto. intros. apply H; auto. eright. apply H3.
+      - apply IHepsilon_; auto. intros. apply H; auto. econstructor 2. apply H3.
+      - apply IHepsilon_; auto. intros. apply H; auto. econstructor 3. apply H3.
     Qed.
 
-    Lemma ss_epsilon_r {E F C D X Y L R} `{Stuck: B0 -< C} `{Stuck': B0 -< D}
+    Lemma ss_epsilon_r {E F C D X Y L R}
         (t : ctree E C X) (u u0 : ctree F D Y) :
       epsilon u u0 ->
       ss L R t u0 ->
@@ -415,7 +449,7 @@ Helper inductive: [epsilon t t'] judges that [t'] is reachable from [t] by a pat
       eapply epsilon_trans in H1; eauto.
     Qed.
 
-    Lemma ssim_epsilon_l {E F C D X Y L} `{Stuck: B0 -< C} `{Stuck': B0 -< D}
+    Lemma ssim_epsilon_l {E F C D X Y L}
         (t0 t : ctree E C X) (u : ctree F D Y) :
       epsilon t0 t ->
       ssim L t0 u ->
@@ -425,7 +459,7 @@ Helper inductive: [epsilon t t'] judges that [t'] is reachable from [t] by a pat
       step in H0. step. eapply ss_epsilon_l in H0; eauto.
     Qed.
 
-    Lemma ssim_epsilon_l' {E F C D X Y L} `{Stuck: B0 -< C} `{Stuck': B0 -< D}
+    Lemma ssim_epsilon_l' {E F C D X Y L}
         (t : ctree E C X) (u : ctree F D Y) :
       (forall t0, epsilon t t0 -> productive t0 -> ssim L t0 u) ->
       ssim L t u.
@@ -434,7 +468,7 @@ Helper inductive: [epsilon t t'] judges that [t'] is reachable from [t] by a pat
       intros. apply H in H1. now step in H1. assumption.
     Qed.
 
-    Lemma ssim_epsilon_r {E F C D X Y L} `{Stuck: B0 -< C} `{Stuck': B0 -< D}
+    Lemma ssim_epsilon_r {E F C D X Y L}
         (t : ctree E C X) (u u0 : ctree F D Y) :
       epsilon u u0 ->
       ssim L t u0 ->
@@ -444,24 +478,24 @@ Helper inductive: [epsilon t t'] judges that [t'] is reachable from [t] by a pat
       step in H0. step. eapply ss_epsilon_r in H0; eauto.
     Qed.
 
-    Lemma ssim_ret_epsilon {E F C D X Y L} `{HasB0: B0 -< C} `{HasB0': B0 -< D} :
+    Lemma ssim_ret_epsilon {E F C D X Y L} :
       forall r (u : ctree F D Y),
       Respects_val L ->
       (Ret r : ctree E C X) (≲L) u ->
       exists r', epsilon u (Ret r') /\ L (val r) (val r').
     Proof.
       intros * RV SIM *.
-      step in SIM. specialize (SIM (val r) stuckD (trans_ret _)).
+      step in SIM. specialize (SIM (val r) Stuck (trans_ret _)).
       destruct SIM as (l' & u' & TR & _ & EQ).
       apply RV in EQ as ?. destruct H as [? _]. specialize (H (Is_val _)). inv H.
       apply trans_val_invT in TR as ?. subst.
       apply trans_val_epsilon in TR as []. eauto.
     Qed.
 
-    Lemma ssim_vis_epsilon {E F C D X Y Z L} `{HasB0: B0 -< C} `{HasB0': B0 -< D} :
+    Lemma ssim_vis_epsilon {E F C D X Y Z L} :
       forall e (k : Z -> ctree E C X) (u : ctree F D Y),
       Respects_val L ->
-      Respects_tau L ->
+      Respects_τ L ->
       Vis e k (≲L) u ->
       forall x, exists Z' (e' : F Z') k' y, epsilon u (Vis e' k') /\ k x (≲L) k' y /\ L (obs e x) (obs e' y).
     Proof.
@@ -482,15 +516,16 @@ Helper inductive: [epsilon t t'] judges that [t'] is reachable from [t] by a pat
       eexists _, _, _, _. etrans.
     Qed.
 
-    Lemma ssim_brS_epsilon {E F C D X Y Z L} `{HasB0: B0 -< C} `{HasB0': B0 -< D} :
+    Lemma ssim_brS_epsilon {E F C D X Y Z L} :
       forall c (k : Z -> ctree E C X) (u : ctree F D Y),
-      Respects_tau L ->
-      L tau tau ->
+      Respects_τ L ->
+      L τ τ ->
       BrS c k (≲L) u ->
-      forall x, exists Z' (c' : D Z') k' y, epsilon u (BrS c' k') /\ k x (≲L) k' y.
+      forall x,
+      (exists v, epsilon u (Step v) /\ k x (≲L) v).
     Proof.
       intros * RT HL SIM *.
-      step in SIM. cbn in SIM. specialize (SIM tau (k x) (trans_brS _ _ _)).
+      step in SIM. cbn in SIM. specialize (SIM τ (k x) (trans_brS _ _ _)).
       destruct SIM as (l' & u'' & TR & SIM & EQ).
       apply trans_epsilon in TR. destruct TR as (u' & EPS & PROD & TR).
       destruct PROD.
@@ -502,8 +537,9 @@ Helper inductive: [epsilon t t'] judges that [t'] is reachable from [t] by a pat
         subs. inv_trans. subst.
         apply RT in EQ. destruct EQ as [? _]. specialize (H eq_refl). inv H.
       }
-      subs. inv_trans. subst.
-      eexists _, _, _, _. etrans.
+      subs.
+      inv_trans. subst.
+      eexists _. etrans.
     Qed.
 
   End epsilon_theory.
